src/study/Nemonuri.Study.CSharpSyntaxRewriter2.Modifier/Nemonuri.StratifiedNode.IndexTheory.Properties.fst
@@ -1,0 +1,4 @@
+module Nemonuri.StratifiedNode.IndexTheory.Properties
+
+open Nemonuri.StratifiedNode.IndexTheory.Base
+
