src/study/Nemonuri.Study.CSharpSyntaxRewriter2.Modifier/Nemonuri.StratifiedNode.IndexTheory.fst
@@ -1,0 +1,4 @@
+module Nemonuri.StratifiedNode.IndexTheory
+
+include Nemonuri.StratifiedNode.IndexTheory.Base
+include Nemonuri.StratifiedNode.IndexTheory.Properties
